splitting/splitting_ltac2_tactics.v
@@ -1,0 +1,211 @@
+From iris.bi Require Export bi telescopes.
+From iris.proofmode Require Export base classes notation.
+Set Default Proof Using "Type".
+
+From Local Require Import named_prop.
+From Local Require Import connection.
+
+From Ltac2 Require Import Ltac2.
+
+From Local Require utils.
+Import utils.Misc utils.Iriception utils.Evars.
+
+From Local Require ltac2_tactics.
+From Local Require Import splitting_tactics.
+
+
+Require Import Ltac2.Std.
+
+(* getting them from
+  Ltac2 Notation "test" s(strategy) := s.
+  Ltac2 Eval (test). *)
+
+Ltac2 Type ident_ltac2 := constr.
+Ltac2 red_flags_default := { rBeta := true; rMatch := true; rFix := true; rCofix := true; rZeta := true; rDelta := true; rConst := [] }.
+
+Ltac2 new_constraint () := new_evar_with_cast '(bool).
+
+Ltac2 rec unify_with_bool (e : constr) (b : bool) :=
+  let er := Std.eval_cbn red_flags_default e in
+  lazy_match! er with
+  | negb ?b0 => unify_with_bool b0 (Bool.neg b)
+  | andb ?b1 ?b2 =>
+    unify_with_bool b1 b;
+    match b with
+    | true => unify_with_bool b2 true
+    | false => ()
+    end
+  | orb ?b1 ?b2 =>
+    match b with
+    | false => unify_with_bool b1 false
+    | true => unify_with_bool b1 true; unify_with_bool b1 true
+    end
+  | ?b0 =>
+     let br := match b with true => '(true) | false => '(false) end in
+     unify0 b0 br
+  end.
+
+Ltac2 rec unify_constr_true (e : constr) := unify_with_bool e true.
+
+
+Ltac2 rec unify_constr_false (e : constr) := unify_with_bool
+
+Ltac2 pm_reduce () :=
+  cbv [named_prop.get_ident
+       connection.translate_envs connection.translate_env
+       named_prop.env_lookup named_prop.env_lookup_with_constr
+       named_prop.env_lookup_true
+       named_prop.env_delete
+       named_prop.env_app named_prop.env_replace
+       named_prop.env_intuitionistic named_prop.env_spatial
+       named_prop.env_counter named_prop.env_spatial_is_nil
+       named_prop.env_Forall
+       named_prop.envs_lookup named_prop.envs_lookup_with_constr
+       named_prop.envs_lookup_true
+       named_prop.envs_delete
+       named_prop.envs_snoc named_prop.envs_app
+       named_prop.envs_simple_replace named_prop.envs_replace
+       named_prop.envs_split named_prop.envs_clear_spatial
+       named_prop.envs_clear_intuitionistic named_prop.envs_incr_counter
+       named_prop.envs_split];
+  ltac2_tactics.pm_reduce ().
+
+Ltac2 pm_reflexivity () :=
+  pm_reduce (); exact eq_refl.
+
+Ltac2 pm_prettify () :=
+  ltac2_tactics.pm_prettify ().
+
+Ltac2 i_solve_tc := ltac2_tactics.i_solve_tc.
+
+Ltac2 i_start_split_proof () :=
+  let apply_named () := refine '(from_named _ _ _) > [ pm_reduce ()] in
+  lazy_match! goal with
+  | [|- @environments.envs_entails _ _ _] => apply_named ()
+  | [|- @envs_entails _ _ _] => ()
+  | [|- ?p ] => ltac2_tactics.i_start_proof (); apply_named ()
+  end.
+
+
+Ltac2 i_fresh_fun () :=
+  i_start_split_proof ();
+  lazy_match! goal with
+   | [|- @envs_entails ?pr1 (@Envs ?pr2 ?p ?s ?c) ?q] =>
+    (ltac1:(pr1 pr2 p s c q |-
+           let c1 := (eval vm_compute in (Pos.succ c)) in
+           change_no_check (@envs_entails pr1 (@Envs pr2 p s c1) q))
+           (Ltac1.of_constr pr1) (Ltac1.of_constr pr2) (Ltac1.of_constr p) (Ltac1.of_constr s) (Ltac1.of_constr c) (Ltac1.of_constr q));
+     constr:(IAnon $c)
+end.
+
+Ltac2 i_intro_pat' (x : Std.intro_pattern) :=
+  or (fun () => failwith (fun () => intros0 false [x]) "couldn't use intro")
+     (fun () =>
+      failwith i_start_split_proof "couldn't start proof in i_intro_pat";
+      lazy_match! goal with
+      | [|- @envs_entails _ _ _] =>
+        refine '(tac_forall_intro _ _ _ _ _) >
+        [ () | ()
+        | orelse i_solve_tc
+          (fun e => lazy_match! goal with
+           | [|- FromForall ?p _ : _] =>
+             Control.zero (Iriception
+                             ((Message.of_string "iIntro: cannot turn ") ++
+                              (Message.of_constr p) ++
+                              (Message.of_string " into a universal quantifier")))
+           end)
+        | pm_prettify (); intros0 false [x] ]
+      end).
+
+Ltac2 Notation "i_intro_pat" p(intropattern) := i_intro_pat' p.
+
+Ltac2 i_intro_ident (x: ident_ltac2) :=
+  failwith (i_start_split_proof) "Couldn't start splitting proof in intro_constr";
+  or
+    (fun () => refine '(@tac_impl_intro _ _ $x _ _ _ _ _ _ _ _) >
+            [() | () | ()
+            | i_solve_tc ()
+            | pm_reduce (); ltac2_tactics.i_solve_tc ()
+            | i_solve_tc ()
+            | pm_reduce ();
+              lazy_match! goal with
+              | [|- False] => Control.zero (Iriception (os "i_intro " ++ oc x ++ os " not fresh"))
+              | [|- _] => ()
+               end])
+    (fun () => refine '(@tac_wand_intro _ _ $x _ _ _ _ _) >
+            [ () | ()
+            | i_solve_tc ()
+            | pm_reduce ()]).
+
+Ltac2 i_intro_intuitionistic_ident (x : ident_ltac2) :=
+  failwith (i_start_split_proof)
+           "Couldn't start splitting proof in intro_constr";
+    or (fun () =>
+        refine '(tac_impl_intro_intuitionistic _ $x _ _ _ _ _ _ _) >
+        [ () | () | ()
+        | i_solve_tc () | i_solve_tc ()
+        | pm_reduce ()])
+     (fun () =>
+        refine '(tac_wand_intro_intuitionistic _ $x _ _ _ _ _ _ _ _) >
+        [ () | () | ()
+        | i_solve_tc () | i_solve_tc ()
+        | i_solve_tc () | pm_reduce ()]).
+
+Ltac2 i_exact_spatial h :=
+  let rec list_from_env e :=
+      match! e with
+      | Esnoc ?gg (?b,?j) ?pp =>
+        match (Constr.equal h j) with
+        | true => unify_constr_true b; list_from_env gg
+        | false => b :: list_from_env gg
+        end
+      | Enil => []
+      end in
+  lazy_match! goal with
+  | [|- @envs_entails _ (@Envs _ ?gp ?gs _) ?q] =>
+    let list_of_constr := list_from_env gs in
+    List.iter (fun b => unify_constr_false b) list_of_constr
+  end;
+  refine '(tac_assumption _ $h _ _ _ _ _ _) >
+  [() | () | pm_reflexivity ()
+  | i_solve_tc ()
+  | pm_reduce (); i_solve_tc ()].
+
+Ltac2 i_and_destruct (x : ident_ltac2)
+                     (y : ident_ltac2)
+                     (z : ident_ltac2) :=
+  refine '(tac_and_destruct _ $x _ $y $z _ _ _ _ _ _ _ _).
+
+
+Ltac2 rec env_length (x : constr) :=
+  lazy_match! x with
+  | Enil => 0
+  | Esnoc ?x _ _ => Int.add 1 (env_length x)
+  end.
+
+Ltac2 i_split () :=
+  let n :=
+    lazy_match! goal with
+    | [|- @envs_entails _ (@Envs _ ?gp ?gs _) ?q] => env_length gs
+    end in
+  let rec gen_list n :=
+    match (Int.equal 0 n) with
+    | true => '(nil)
+    | false =>
+      let v := new_constraint () in
+      let tl := gen_list (Int.sub n 1) in
+      '($v :: $tl)
+    end in
+  let bs := gen_list n in
+  match! goal with
+  | [|- @envs_entails _ ?g ?q] =>
+    refine '(tac_sep_split $g $bs _ _ _ _ _) >
+    [ () | ()
+    | i_solve_tc ()
+    | pm_reduce ();
+      lazy_match! goal with
+      | [ |- False] => iriception "couldn't split the context"
+      | [ |- _] => split > [() | ()]
+      end]
+  | [|- _] => iriception "the goal isn't bi entailment"
+  end.
